specIR/SIR3.v
@@ -1,0 +1,260 @@
+From Coq Require Import
+     Arith.PeanoNat
+     Lists.List
+     Strings.String
+     Morphisms
+     Setoid
+     RelationClasses.
+
+Require Import MapsC.
+Require Import ValuesC.
+Require Import MemoryC.
+Require Import CoqlibC.
+Require Import ASTC.
+Require Import EventsC.
+Require Import GlobalenvsC.
+Require Import IntegersC.
+Require Import Mod ModSem Any Skeleton.
+Require Import SIRCommon.
+
+Require Import Program.
+
+Set Implicit Arguments.
+
+
+
+
+Section OWNEDHEAP.
+
+Variable owned_heap: Type.
+
+Let eff1: Type -> Type := eff1 owned_heap.
+Let eff2: Type -> Type := eff2 owned_heap.
+Let eff3: Type -> Type := eff3 owned_heap.
+Let eff4: Type -> Type := eff4 owned_heap.
+Let eff5: Type -> Type := eff5 owned_heap.
+Let E: Type -> Type := E owned_heap.
+Let OwnedHeapE: Type -> Type := OwnedHeapE owned_heap.
+Let program: Type := program owned_heap.
+Let fn_sig := @fn_sig owned_heap.
+
+Section MODSEM.
+
+  Variable mi: string.
+  Variable skenv_link: SkEnv.t.
+  Variable initial_owned_heap: owned_heap.
+  Variable p: program.
+  Let skenv: SkEnv.t := (SkEnv.project skenv_link) (Sk.of_program fn_sig p).
+  (* Let ge: genv := (SkEnv.revive skenv) p. *)
+  Definition genvtype: Type := unit.
+  Let ge: genvtype := tt.
+
+  Record state := mk {
+    itr:> itree eff3 val;
+    le: lenv;
+    oh: owned_heap;
+    m: mem;
+  }.
+
+  Let denote_program3 := denote_program3 p skenv.
+
+  Inductive initial_frame (oh0: owned_heap) (args: Args.t): state -> Prop :=
+  | initial_frame_intro
+      fid blk m0 vs itr fd tvs
+      (FPTR: (Args.fptr args) = Vptr blk Ptrofs.zero)
+      (VS: (Args.vs args) = vs)
+      (M: (Args.m args) = m0)
+
+      (SYMB: Genv.find_symbol skenv fid = Some blk)
+      (FINDF: Genv.find_funct skenv (Vptr blk Ptrofs.zero) = Some (Internal fd))
+      (TYP: typecheck (Args.vs args) fd tvs)
+      (DENOTE: denote_program3 (ICall fid vs) = itr)
+
+      st0
+      (ST: st0 = (mk itr nil oh0 m0))
+    :
+      initial_frame oh0 args st0
+  .
+
+  Inductive at_external (st0: state): owned_heap -> Args.t -> Prop :=
+  | at_external_intro
+      args fptr vs k
+      (VIS: (observe st0) = VisF (subevent _ (ECall fptr vs)) k)
+      (ARGS: args = Args.mk fptr vs st0.(m))
+    :
+      at_external st0 st0.(oh) args
+  .
+
+  Inductive get_k (st0: state): (val -> itree eff3 val) -> Prop :=
+  | get_k_intro
+      _vs _fptr k
+      (VIS: (observe st0) = VisF (subevent _ (ECall _fptr _vs)) k)
+    :
+      get_k st0 k
+  .
+
+  Inductive after_external (st0: state) (oh0: owned_heap) (retv: Retv.t): state -> Prop :=
+  | after_external_intro
+      k m0 rv st1
+      (GETK: get_k st0 k)
+      (V: (Retv.v retv) = rv)
+      (M: (Retv.m retv) = m0)
+      (KONT: st1 = mk (k rv) st0.(le) oh0 m0)
+    :
+      after_external st0 oh0 retv st1
+  .
+
+  Inductive final_frame (st0: state): owned_heap -> Retv.t -> Prop :=
+  | final_frame_intro
+      oh0 m0 (rv: val) retv
+      (RET: (observe st0) = RetF rv)
+      (RETV: retv = Retv.mk rv m0)
+      (M: m0 = st0.(m))
+      (OH: oh0 = st0.(oh))
+    :
+      final_frame st0 oh0 retv
+  .
+
+  Inductive step (se: Senv.t) (ge: genvtype) (st0: state) (tr: trace) (st1: state): Prop :=
+  | step_tau
+      itr0 le0 oh0 m0
+      itr1
+      (TAU: (observe itr0) = TauF itr1)
+
+      (ST0: st0 = mk itr0 le0 oh0 m0)
+      (TR: tr = E0)
+      (ST1: st1 = mk itr1 le0 oh0 m0)
+  (*** ub is stuck, so we don't state anything ***)
+  | step_nb
+      msg k
+      (VIS: (observe st0) = VisF (subevent _ (ENB msg)) k)
+
+      (TR: tr = E0)
+  | step_syscall
+      itr0 le0 oh0 m0
+      ef vs rv m1 k
+      (VIS: (observe st0) = VisF (subevent _ (ESyscall ef vs)) k)
+      (SYSCALL: external_call ef se vs m0 tr rv m1)
+
+      (ST0: st0 = mk itr0 le0 oh0 m0)
+      (TR: tr = E0)
+      (ST1: st1 = mk (k rv) le0 oh0 m1)
+  | step_done
+      itr0 le0 oh0 m0
+      v k
+      (VIS: (observe st0) = VisF (subevent _ (EDone v)) k)
+
+      (ST0: st0 = mk itr0 le0 oh0 m0)
+      (TR: tr = E0)
+      (ST1: st1 = mk (Ret v) le0 oh0 m0)
+  | step_mget
+      itr0 le0 oh0 m0
+      k
+      (VIS: (observe st0) = VisF (subevent _ (Get _)) k)
+
+      (ST0: st0 = mk itr0 le0 oh0 m0)
+      (TR: tr = E0)
+      (ST1: st1 = mk (k m0) le0 oh0 m0)
+  | step_mput
+      itr0 le0 oh0 m0
+      m1 k
+      (VIS: (observe st0) = VisF (subevent _ (Put _ m1)) k)
+
+      (ST0: st0 = mk itr0 le0 oh0 m0)
+      (TR: tr = E0)
+      (ST1: st1 = mk (k tt) le0 oh0 m1)
+  | step_ohget
+      itr0 le0 oh0 m0
+      k
+      (VIS: (observe st0) = VisF (subevent _ (Get _)) k)
+
+      (ST0: st0 = mk itr0 le0 oh0 m0)
+      (TR: tr = E0)
+      (ST1: st1 = mk (k oh0) le0 oh0 m0)
+  | step_ohput
+      itr0 le0 oh0 m0
+      oh1 k
+      (VIS: (observe st0) = VisF (subevent _ (Put _ oh1)) k)
+
+      (ST0: st0 = mk itr0 le0 oh0 m0)
+      (TR: tr = E0)
+      (ST1: st1 = mk (k tt) le0 oh1 m0)
+  | step_lget
+      itr0 (hd0: ident -> option val) (tl0: lenv) oh0 m0
+      k x v
+      (VIS: (observe st0) = VisF (subevent _ (LGet x)) k)
+      (GET: hd0 x = Some v)
+
+      (ST0: st0 = mk itr0 (hd0 :: tl0) oh0 m0)
+      (TR: tr = E0)
+      (ST1: st1 = mk (k v) (hd0 :: tl0) oh0 m0)
+  | step_lput
+      itr0 (hd0: ident -> option val) (tl0: lenv) oh0 m0
+      x v k
+      (VIS: (observe st0) = VisF (subevent _ (LPut x v)) k)
+
+      (ST0: st0 = mk itr0 (hd0 :: tl0) oh0 m0)
+      (TR: tr = E0)
+      (ST1: st1 = mk (k tt) (Maps.add x v hd0 :: tl0) oh0 m0)
+  | step_lpush
+      itr0 le0 oh0 m0
+      k
+      (VIS: (observe st0) = VisF (subevent _ (LPush)) k)
+
+      (ST0: st0 = mk itr0 le0 oh0 m0)
+      (TR: tr = E0)
+      (ST1: st1 = mk (k tt) (Maps.empty :: le0) oh0 m0)
+  | step_lpop
+      itr0 (hd0: ident -> option val) (tl0: lenv) oh0 m0
+      k
+      (VIS: (observe st0) = VisF (subevent _ (LPop)) k)
+
+      (ST0: st0 = mk itr0 (hd0 :: tl0) oh0 m0)
+      (TR: tr = E0)
+      (ST1: st1 = mk (k tt) (tl0) oh0 m0)
+  .
+
+  Program Definition modsem: ModSem.t :=
+    {| ModSem.step := step;
+       ModSem.owned_heap := owned_heap;
+       ModSem.at_external := at_external;
+       ModSem.initial_frame := initial_frame;
+       ModSem.final_frame := final_frame;
+       ModSem.after_external := after_external;
+       ModSem.initial_owned_heap := initial_owned_heap;
+       ModSem.globalenv := ge;
+       ModSem.skenv := skenv;
+       ModSem.skenv_link := skenv_link;
+       ModSem.midx := Some mi;
+    |}.
+  Next Obligation.
+    inv AT0. inv AT1. rewrite VIS in *. clarify.
+  Qed.
+  Next Obligation.
+    inv FINAL0. inv FINAL1. rewrite RET in *. clarify.
+  Qed.
+  Next Obligation.
+    inv AFTER0. inv AFTER1. inv GETK. inv GETK0. rewrite VIS in *.
+    ss. clarify. simpl_depind. clarify.
+  Qed.
+  Next Obligation.
+    ii. des. inv PR; ss. inv PR0; ss; clarify; try rewrite VIS in *; ss; clarify.
+  Qed.
+  Next Obligation.
+    ii. des. inv PR0; ss. inv PR; ss; clarify; try rewrite RET in *; ss; clarify.
+  Qed.
+  Next Obligation.
+    ii. des. inv PR; ss. inv PR0; ss; clarify; try rewrite VIS in *; ss; clarify.
+  Qed.
+
+End MODSEM.
+
+Program Definition module (p: program) (mi: string) (initial_owned_heap: SkEnv.t -> owned_heap): Mod.t :=
+  {| Mod.data := p; Mod.get_sk := (Sk.of_program fn_sig);
+     Mod.get_modsem := fun skenv_link p => modsem mi skenv_link
+                                                  (initial_owned_heap skenv_link) p;
+     Mod.midx := Some mi |}
+.
+
+End OWNEDHEAP.
+
