specIR/SIRProps.v
@@ -1,0 +1,84 @@
+From Coq Require Import
+     Arith.PeanoNat
+     Lists.List
+     Strings.String
+     Morphisms
+     Setoid
+     RelationClasses.
+
+Require Import MapsC.
+Require Import ValuesC.
+Require Import MemoryC.
+Require Import CoqlibC.
+Require Import ASTC.
+Require Import EventsC.
+Require Import GlobalenvsC.
+Require Import IntegersC.
+Require Import Mod ModSem Any Skeleton SimMod SimModSem.
+Require Import Sound SoundTop SimMem SimMemId SimSymb.
+Require Import SIRCommon SIR2 SIR3.
+
+Require Import Program.
+
+Set Implicit Arguments.
+
+
+
+Local Existing Instance SimMemOh_default.
+Global Arguments ModSemPair.mk [SM] [SS] _ _ _ _ [SMO].
+
+Section OWNEDHEAP.
+
+Variable owned_heap: Type.
+Variable initial_owned_heap: SkEnv.t -> owned_heap.
+
+
+
+
+
+Section SIMMODSEM.
+
+Variable skenv_link: SkEnv.t.
+Variable sm_link: SimMem.t.
+Variable prog: program owned_heap.
+Variable mi: string.
+Let md_src: Mod.t := (SIR2.module prog mi initial_owned_heap).
+Let md_tgt: Mod.t := (SIR3.module prog mi initial_owned_heap).
+Hypothesis (INCLSRC: SkEnv.includes skenv_link (Mod.sk md_src)).
+Hypothesis (INCLTGT: SkEnv.includes skenv_link (Mod.sk md_tgt)).
+Hypothesis (WF: SkEnv.wf skenv_link).
+
+Definition msp: ModSemPair.t := ModSemPair.mk (md_src skenv_link) (md_tgt skenv_link)
+                                              (SimSymbId.mk md_src md_tgt) sm_link.
+
+Print SIR2.state.
+Print SIR3.state.
+
+Theorem sim_modsem: ModSemPair.sim msp.
+Proof.
+  econs; eauto.
+Qed.
+
+End SIMMODSEM.
+
+
+
+
+
+Section SIMMOD.
+
+Variable prog: program owned_heap.
+Variable mi: string.
+
+Definition mp: ModPair.t := SimSymbId.mk_mp (SIR0.module prog mi initial_owned_heap)
+                                            (SIR2.module prog mi initial_owned_heap).
+
+Theorem sim_mod: ModPair.sim mp.
+Proof.
+  econs; ss.
+  - ii. inv SIMSKENVLINK. eexists. eapply sim_modsem; eauto.
+Qed.
+
+End SIMMOD.
+
+End OWNEDHEAP.
